snapshot

src/Framework/SemSubstDefunc.v
@@ -5,15 +5,9 @@ From CertiCoq.Libraries Require Import maps_util.
 Import ListNotations.
 Require Import Lia.
 
-From Framework Require Import Util ANF SemSubst.
+From Framework Require Import Util ANF Exposed.
 
 (* Defunc
-
-[[ let gf = fun [w_gf] () {f_work}
-   let t = gf [w_gf] ()
-   in case [w_work] t
-      C => let t' = proj [w_work] t in t'
-      ... ]]
 
 let f_wrap = fun [w_wrap] (x) ->
                 let f_work = C [w_work] f_wrap
@@ -55,3 +49,254 @@ let h = fun [w_h] (f') ->
 in h [w_h] f
 
 *)
+
+(* Map f_wrap to the corresponding constructor *)
+Definition trans_info_t := M.t ctor_tag.
+
+Definition wrapper_info_t := unit.
+
+Module LT <: Exposed.LTy. Definition t : Type := (trans_info_t * wrapper_info_t * web). End LT.
+Module LM := Exposed.DefaultL LT.
+Export LM.
+
+Definition tail_cases (cs : list (var * ctor_tag)) f_work w_work :=
+  List.map (fun (p : var * ctor_tag) =>
+              let (c, f_wrap) := p in
+              (c, Eproj f_wrap w_work 0 f_work (* project out the function *)
+                    (Eret f_wrap))) (* ret it *)
+    cs.
+
+Definition wrap
+  (C : trans_info_t) (_ : wrapper_info_t)
+  (f_work : var) (w_work : web)
+  (f_wrap : var) (w_wrap : web) : exp :=
+  Ecase f_work w_work (tail_cases (M.elements C) f_work w_work).
+
+Definition values {A} (m : M.t A) : list A :=
+  List.map snd (M.elements m).
+
+Definition wrap_prop
+  (C : trans_info_t) (_ : wrapper_info_t)
+  (f_work : var) (w_work : web)
+  (f_wrap : var) (w_wrap : web) : Prop :=
+  NoDup (values C).
+
+(* Specification *)
+Inductive trans (Γ : Ensemble var) : exp -> exp -> Prop :=
+| Trans_fun :
+  forall {f f_wrap w xs C u c e k e' k' f_temp w_temp w_wrap},
+    let wrapper := (wrap C u f w f_wrap w_wrap) in
+
+    trans (FromList xs :|: (f |: Γ)) e e' ->
+    trans (f |: Γ) k k' ->
+
+    (* worker spec *)
+    L ! w = None ->
+    (~ w \in Exposed) ->
+    (~ In f xs) ->
+    (~ f \in bound_var wrapper) ->
+
+    (* temp binder spec *)
+    L ! w_temp = None ->
+    (~ w_temp \in Exposed) ->
+    (~ f_temp \in (occurs_free e)) ->
+    (~ f_temp \in (occurs_free k)) ->
+    (~ f_temp \in Γ) ->
+    f_temp <> f ->
+    (~ In f_temp xs) ->
+
+    (* wrapper spec *)
+    L ! w_wrap = Some (C, u, w) ->
+    wrap_prop C u f w f_wrap w_wrap ->
+    C ! f_wrap = Some c ->
+
+    trans Γ (Efun f_wrap w_wrap xs
+               (Econstr f w c [f_wrap]
+                  (Efun f_temp w_temp [] wrapper
+                     (Eletapp f f_temp w_temp [] e)))
+               (Econstr f w c [f_wrap]
+                  (Efun f_temp w_temp [] wrapper
+                     (Eletapp f f_temp w_temp [] k))))
+      (Efun f_wrap w_wrap xs
+         (Econstr f w c [f_wrap] e')
+         (Econstr f w c [f_wrap] k')) (* turn the wrapper into the worker *)
+
+| Trans_app :
+  forall {C u f w xs f_temp w_temp f_wrap w_wrap},
+    let wrapper := (wrap C u f w f_wrap w_wrap) in
+
+    (f \in Γ) ->
+    (FromList xs \subset Γ) ->
+
+    (* worker spec *)
+    L ! w = None ->
+    (~ w \in Exposed) ->
+    (~ f \in bound_var wrapper) ->
+
+    (* temp binder spec *)
+    L ! w_temp = None ->
+    (~ w_temp \in Exposed) ->
+    f_temp <> f ->
+    (~ In f_temp xs) ->
+
+    (* wrapper spec *)
+    L ! w_wrap = Some (C, u, w) ->
+    wrap_prop C u f w f_wrap w_wrap ->
+
+    trans Γ (Eapp f w_wrap xs)
+      (Efun f_temp w_temp [] wrapper
+         (Eletapp f_temp f_temp w_temp [] (* turn the worker into the wrapper *)
+            (Eapp f_temp w_wrap xs))).
+
+Hint Constructors trans : core.
+
+(*
+Lemma free_vars_wrap C u w_work f_wrap w_wrap f:
+  let wrapper := (wrap C u f w_work f_wrap w_wrap) in
+  (~ f \in (bound_var wrapper)) ->
+  (occurs_free wrapper <--> [set f]).
+Proof.
+  unfold wrap, Same_set, Ensembles.Included, Ensembles.In.
+  intro cs.
+  induction cs; simpl; split; intros.
+  - inv H0; constructor.
+  - inv H0; auto.
+  - inv H0; try constructor.
+    + inv H7; try constructor.
+      inv H8; contradiction.
+    + destruct IHcs; eauto.
+      intros Hc.
+      apply H.
+      inv Hc.
+      eapply Bound_Ecase; eauto.
+      eapply in_cons; eauto.
+  - inv H0; auto.
+Qed.
+ *)
+
+
+(* Logical Relations *)
+Module VTransM <: Exposed.VTrans LM.
+
+  (* Relating wrapper and worker *)
+  Definition V_trans
+    (V' : nat -> wval -> wval -> Prop)
+    (E' : nat -> env -> exp -> env -> exp -> Prop)
+    (i0 : nat) (d : trans_info_t * wrapper_info_t * web)
+    (w_wrap : web) (v_wrap : val) (w_work' : web) (v_work : val) :=
+    let '(C, u, w_work) := d in
+    w_work = w_work' /\
+    match v_wrap with
+    | Vfun f1 ρ1 xs1 e1 =>
+        forall f_work f_wrap ρ,
+          let wrapper := (wrap C u f_work w_work f_wrap w_wrap) in
+          (~ f_work \in bound_var wrapper) ->
+          wf_env ρ ->
+
+          exists k ρ2 xs2 e2,
+            bstep_fuel false (M.set f_work (Tag w_work v_work) ρ) wrapper k (Res (Tag w_wrap (Vfun f_wrap ρ2 xs2 e2))) /\
+            length xs1 = length xs2 /\
+
+            forall j vs1 vs2 ρ3 ρ4,
+              j <= i0 ->
+              Forall wf_val vs1 ->
+              Forall2 (V' j) vs1 vs2 ->
+              set_lists xs1 vs1 (M.set f1 (Tag w_wrap (Vfun f1 ρ1 xs1 e1)) ρ1) = Some ρ3 ->
+              set_lists xs2 vs2 (M.set f_wrap (Tag w_wrap (Vfun f_wrap ρ2 xs2 e2)) ρ2) = Some ρ4 ->
+              E' j ρ3 e1 ρ4 e2
+
+    | _ => False
+    end.
+
+  Lemma V_trans_mono V E i j d w1 v1 w2 v2 :
+    (forall k : nat,
+        k < S i ->
+        forall (j : nat) (v1 v2 : wval), V k v1 v2 -> j <= k -> V j v1 v2) ->
+    V_trans (fun i' => V (i - (i - i'))) (fun i' => E (i - (i - i'))) i d w1 v1 w2 v2 ->
+    j <= i ->
+    V_trans (fun j' => V (j - (j - j'))) (fun j' => E (j - (j - j'))) j d w1 v1 w2 v2.
+  Proof.
+    intros HI. intros.
+    destruct v1; auto;
+      simpl in *; try contradiction.
+      rename l into xs1.
+    unfold V_trans in *.
+    destruct d.
+    destruct p.
+    destruct H as [Hw HV]; subst.
+    repeat split; eauto; intros.
+    edestruct (HV f_work f_wrap ρ) as [k [ρ2 [xs2 [e2 [Hstep [Hlen HV']]]]]]; eauto.
+    exists k, ρ2, xs2, e2; repeat (split; auto); intros.
+    specialize (HV' j0 vs1 vs2 ρ3 ρ4).
+    rewrite normalize_step in *; try lia.
+    eapply HV'; eauto; try lia.
+  Qed.
+
+End VTransM.
+
+Import VTransM ExposedUtil.
+
+Module EM := Exposed.Exposed LM VTransM.
+Import EM.
+
+(* Compatibility Lemmas *)
+Lemma fun_compat_trans Γ1 e e' C u c k k' f w xs w_temp f_temp w_wrap f_wrap :
+  let wrapper := (wrap C u f w f_wrap w_wrap) in
+  trans_correct (FromList xs :|: (f |: Γ1)) e e' ->
+  occurs_free e' \subset occurs_free e ->
+
+  trans_correct (f |: Γ1) k k' ->
+  occurs_free k' \subset occurs_free k ->
+
+  (* worker spec *)
+  M.get w L = None ->
+  (~ w \in Exposed) ->
+  (~ In f xs) ->
+  (~ f \in bound_var wrapper) ->
+
+  (* temp binder spec *)
+  L ! w_temp = None ->
+  (~ w_temp \in Exposed) ->
+  (~ f_temp \in (occurs_free e)) ->
+  (~ f_temp \in (occurs_free k)) ->
+  (~ f_temp \in Γ1) ->
+  f_temp <> f ->
+  (~ In f_temp xs) ->
+
+  (* wrapper spec *)
+  L ! w_wrap = Some (C, u, w) ->
+  wrap_prop C u f w f_wrap w_wrap ->
+  C ! f_wrap = Some c ->
+
+  trans_correct Γ1
+    (Efun f_wrap w_wrap xs
+       (Econstr f w c [f_wrap]
+          (Efun f_temp w_temp [] wrapper
+             (Eletapp f f_temp w_temp [] e)))
+       (Econstr f w c [f_wrap]
+          (Efun f_temp w_temp [] wrapper
+             (Eletapp f f_temp w_temp [] k))))
+    (Efun f_wrap w_wrap xs
+       (Econstr f w c [f_wrap] e')
+       (Econstr f w c [f_wrap] k')).
+Proof.
+  unfold trans_correct, E, E'.
+  intros He Hes Hk Hks Hw Hw1 Hf Hf_bv Hw_temp Hw_temp1 Hf_temp Hf_temp1 Hf_temp2 Hf_temp3 Hf_temp4 Hw_wrap Hwrap_prop HC.
+
+  intros.
+  inv H1.
+  exists 0, OOT; split; simpl; eauto.
+  inv H2.
+
+  inv H10.
+  exists 0, OOT; split; simpl; eauto.
+  inv H1.
+
+  inv H13.
+  exists 0, OOT; split; simpl; eauto.
+  inv H1.
+
+  inv H14.
+  exists 0, OOT; split; simpl; eauto.
+  inv H1.
+  2 : { exists 0, OOT; split; simpl; eauto. }
