src/Framework/SemSubst2.v
@@ -52,55 +52,6 @@ in h1 [w_h1] f
 
 *)
 
-(* Defunc
-
-[[ let gf = fun [w_gf] () {f_work}
-   let t = gf [w_gf] ()
-   in case [w_work] t
-      C => let t' = proj [w_work] t in t'
-      ... ]]
-
-let f_wrap = fun [w_wrap] (x) ->
-                let f_work = C [w_work] f_wrap
-                let g0 = fun [w_g0] () ->
-                           [[ case [w_work] {f_work}
-                              C => let t = proj [w_work] {f_work}
-                                   in t
-                              ... ]]
-                let f = g0 [w_g0] ()
-                in x + 1
-let f_work = C [w_work] f_wrap
-let g1 = fun [w_g1] () ->
-            [[ case [w_work] {f_work}
-               C => let t = proj [w_work] {f_work}
-                    in t
-               ... ]]
-let f = g1 [w_g1] ()
-let h = fun [w_h] (f') -> f' [w_wrap] 0
-in h [w_h] f
-
-~~>
-
-let f_wrap = fun [w_wrap] (x) ->
-                let f_work = C [w_work] f_wrap
-                let g0 = fun [w_g0] () -> f_work
-                let f = g0 [w_g0] ()
-                in x + 1
-let f_work = C [w_work] f_wrap
-let g1 = fun [w_g1] () -> f_work
-let f = g1 [w_g1] ()
-let h = fun [w_h] (f') ->
-          let g2 = fun [w_g2] () ->
-                     case [w_work] f'
-                     C => let t = proj [w_work] f'
-                          in t
-                     ...
-          let f' = g2 [w_g2] ()
-          f' [w_wrap] 0
-in h [w_h] f
-
-*)
-
 (* Map from web identifier to transformation specific information, wrapper specific information, and worker web *)
 Definition trans_info_t := list bool.
 
